src/WFLib.v
@@ -1,4 +1,5 @@
 From sflib Require Import sflib.
+From Paco Require Import paco.
 From Coq Require Export
   Relations.Relation_Operators.
 From Coq Require Import
@@ -222,3 +223,29 @@ Proof.
   i. des. exists (ord_tree_cons f). i.
   exists (f a). splits; eauto. econs; eauto.
 Qed.
+
+
+Section WFTYPE.
+  Record WF: Type :=
+    mk_wf {
+        T: Type;
+        lt: (T -> T -> Prop);
+        wf: well_founded lt;
+        le: (T -> T -> Prop) := eq \2/ lt;
+      }.
+
+  Global Program Instance le_Reflexive {wf: WF}: Reflexive wf.(le).
+  Next Obligation.
+    unfold le. auto.
+  Qed.
+
+  Lemma WF_le_Trans
+        wf
+        (WFTR: Transitive wf.(lt))
+    :
+    Transitive wf.(le).
+  Proof.
+    unfold le. ii. destruct wf; ss. des; clarify; eauto.
+  Qed.
+
+End WFTYPE.
